$\cos(3x+\ang{50;;})=-\cos(2x-\ang{40;;})=\cos(\ang{180;;}-2x+\ang{40;;})$

	Le soluzioni sono
	\[\begin{cases}
	x_1=+\alpha+k\ang{360;;}\\
	x_2=-\alpha+k\ang{360;;}\\
	\end{cases}\]
	Troviamo la prima

	\begin{align*}
	3x+\ang{50;;}&=\ang{180;;}-2x+\ang{40;;}+k\ang{360;;}\\
	3x+2x&=\ang{180;;}-\ang{50;;}+\ang{40;;}+k\ang{360;;}\\
	5x&=\ang{170;;}+k\ang{360;;}\\
	x&=\ang{34;;}+k\ang{72;;}
	\end{align*}
	Troviamo la seconda

	\begin{align*}
		3x+\ang{50;;}&=-\ang{180;;}+2x-\ang{40;;}+k\ang{360;;}\\
		3x-2x&=-\ang{180;;}-\ang{50;;}-\ang{40;;}+k\ang{360;;}\\
		x&=-\ang{270;;}+k\ang{360;;}
	\end{align*}

	Le soluzioni sono

	\[\begin{cases}
	x_1=\ang{34;;}+k\ang{72;;}\\
	x_2-\ang{270;;}+k\ang{360;;}
	\end{cases}\]
