	 $\tan(6x-\ang{30;;})=-\tan(2x-\ang{40;;})=\tan(-2x+\ang{40;;})$

	Esistenza lato sinistro

	\begin{align*}
		6x-\ang{30;;}&=\ang{90;;}+k\ang{180;;}\\
		6x&=\ang{90;;}+\ang{30;;}+k\ang{180;;}\\
		6x&=\ang{120;;}+k\ang{180;;}\\
		x&=\ang{20;;}+k\ang{36;;}
		\end{align*}

	Esistenza lato destro

	\begin{align*}
		-2x+\ang{40;;}&=\ang{90;;}+k\ang{180;;}\\
		-2x&=\ang{90;;}-\ang{40;;}+k\ang{180;;}\\
		-2x&=\ang{50;;}+k\ang{180;;}\\
		x&=-\ang{25;;}+k\ang{90;;}
		\end{align*}
	Troviamo la soluzione

		\begin{align*}
		6x-\ang{30;;}&=-2x+\ang{40;;}+k\ang{180;;}\\
		6x+2x&=\ang{40;;}+\ang{30;;}+k\ang{180;;}\\
		8x&=\ang{70;;}+k\ang{180;;}\\
		x&=\dfrac{\ang{70;;}}{8}+k\dfrac{\ang{180;;}}{8}
		\end{align*}

	La soluzione Ã¨
	\[x=\dfrac{\ang{70;;}}{8}+k\dfrac{\ang{180;;}}{8}\]
